src/arch/x64/X64.Vale.Lemmas_i.fsti
@@ -26,6 +26,10 @@ let eval_ins (c:code) (s0:state) : Ghost ((sM:state) * (f0:fuel))
 
 let eval_ocmp (s:state) (c:ocmp) : bool = S.eval_ocmp (state_to_S s) c
 
+let valid_ocmp (c:ocmp) (s:state) : bool = S.valid_ocmp c (state_to_S s)
+
+let ensure_valid_ocmp (c:ocmp) (s:state) : state = state_of_S (S.run (S.check (S.valid_ocmp c)) (state_to_S s))
+
 val lemma_cmp_eq : s:state -> o1:operand -> o2:operand -> Lemma
   (ensures eval_ocmp s (S.OEq o1 o2) <==> eval_operand o1 s == eval_operand o2 s)
   [SMTPat (eval_ocmp s (S.OEq o1 o2))]
@@ -76,6 +80,7 @@ val lemma_ifElse_total (ifb:ocmp) (ct:code) (cf:code) (s0:state) : Ghost (bool *
 
 val lemma_ifElseTrue_total (ifb:ocmp) (ct:code) (cf:code) (s0:state) (f0:fuel) (sM:state) : Lemma
   (requires
+    valid_ocmp ifb s0 /\
     eval_ocmp s0 ifb /\
     eval_code ct s0 f0 sM
   )
@@ -85,6 +90,7 @@ val lemma_ifElseTrue_total (ifb:ocmp) (ct:code) (cf:code) (s0:state) (f0:fuel) (
 
 val lemma_ifElseFalse_total (ifb:ocmp) (ct:code) (cf:code) (s0:state) (f0:fuel) (sM:state) : Lemma
   (requires
+    valid_ocmp ifb s0 /\
     not (eval_ocmp s0 ifb) /\
     eval_code cf s0 f0 sM
   )
@@ -107,6 +113,7 @@ val lemma_whileTrue_total (b:ocmp) (c:code) (s0:state) (sW:state) (fW:fuel) : Gh
 
 val lemma_whileFalse_total (b:ocmp) (c:code) (s0:state) (sW:state) (fW:fuel) : Ghost ((s1:state) * (f1:fuel))
   (requires
+    valid_ocmp b sW /\
     not (eval_ocmp sW b) /\
     eval_while_inv (While b c) s0 fW sW
   )
@@ -119,6 +126,7 @@ val lemma_whileMerge_total (c:code) (s0:state) (f0:fuel) (sM:state) (fM:fuel) (s
   (requires
     While? c /\
     sN.ok /\
+    valid_ocmp (While?.whileCond c) sM /\
     eval_ocmp sM (While?.whileCond c) /\
     eval_while_inv c s0 f0 sM /\
     eval_code (While?.whileBody c) sM fM sN
